benchmarks/tests.v
@@ -148,8 +148,8 @@ CertiCoq Compile -args 1000 -config 9 -O 1 -ext "_opt_ll" lazy_factorial. *)
 (* CertiCoq Compile -O 1 -cps -ext "_cps_opt" sha. *)
 (* CertiCoq Compile -O 1 -ext "_opt" sha. *)
 
-Eval compute in "Compiling sha_fast".
+(* Eval compute in "Compiling sha_fast". *)
 
-CertiCoq Generate WASM -cps -time -debug sha_fast.
+(* CertiCoq Generate WASM -cps -time -debug sha_fast. *)
 (* CertiCoq Compile -O 0 -cps -ext "_cps" sha_fast. *)
 (* CertiCoq Compile -cps -ext "_cps_opt" sha_fast. *)
